steel/Zeta.Steel.GlobalRel.fsti
@@ -15,6 +15,7 @@ module U64 = FStar.UInt64
 module GG = Zeta.Generic.Global
 module HA = Zeta.Steel.HashAccumulator
 module StT = Zeta.Steel.Thread
+module AH = Zeta.Steel.AggregateEpochHashes
 
 let index_ (logs: all_logs)  (t: tid)
   : tlog
@@ -33,7 +34,7 @@ let index (logs: verifiable_logs) (t: tid)
 (* all verifier threads succeed and have certified upto epmax *)
 let verifiable_and_certified (logs: all_logs) (epmax: epoch_id)
   = verifiable logs /\
-    (forall (eid: epoch_id). (U32.v eid <= U32.v epmax) ==> epoch_is_certified logs eid)
+    (forall (eid: epoch_id). (U32.v eid <= U32.v epmax) ==> AH.epoch_is_certified logs eid)
 
 let n_threads_v = U32.v n_threads
 
@@ -62,11 +63,11 @@ val aggregate_add_hash (logs: all_logs) (ep: epoch_id)
 val aggregate_evict_hash (logs: all_logs) (ep: epoch_id)
   : GTot hash_value_t
 
-val certified_epoch_aggregate_hashes_equal (logs: all_logs) (ep: epoch_id {epoch_is_certified logs ep})
+val certified_epoch_aggregate_hashes_equal (logs: all_logs) (ep: epoch_id {AH.epoch_is_certified logs ep})
   : Lemma (ensures (aggregate_add_hash logs ep = aggregate_evict_hash logs ep))
 
 val aggr_add_hash_correct (logs: verifiable_logs) (ep: epoch_id)
-  : Lemma (requires (epoch_is_certified logs ep))
+  : Lemma (requires (AH.epoch_is_certified logs ep))
           (ensures (let gl = to_ilog logs in
                     let i_ep = lift_epoch ep in
                     let add_set = GG.add_set i_ep gl in
@@ -74,7 +75,7 @@ val aggr_add_hash_correct (logs: verifiable_logs) (ep: epoch_id)
                     h = ms_hashfn add_set))
 
 val aggr_evict_hash_correct (logs: verifiable_logs) (ep: epoch_id)
-  : Lemma (requires (epoch_is_certified logs ep))
+  : Lemma (requires (AH.epoch_is_certified logs ep))
           (ensures (let gl = to_ilog logs in
                     let i_ep = lift_epoch ep in
                     let evict_set = GG.evict_set i_ep gl in
